plugin/runtime/certicoq_run.h
@@ -1,3 +1,0 @@
-#include "values.h"
-
-extern value certicoq_run ();
