plugin/runtime/certicoq_run_wrapper.mli
@@ -1,2 +1,0 @@
-
-val run : Ast0.Env.global_env -> typ:Ast0.term -> Obj.t
