theories/Codegen/toplevel.v
@@ -38,10 +38,10 @@ Definition add_prim_names (prims : list (kername * string * bool * nat * positiv
   List.fold_left (fun map '(k, s, b, ar, p) => cps.M.set p (nNamed s) map) prims nenv.
 
 
-Definition Clight_trans (prims : list (kername * string * bool * nat * positive)) (args : nat) (t : toplevel.LambdaANF_FullTerm) : error Cprogram :=
+Definition Clight_trans (bodyName : string) (prims : list (kername * string * bool * nat * positive)) (args : nat) (t : toplevel.LambdaANF_FullTerm) : error Cprogram :=
   let '(_, p_env, cenv, ctag, itag, nenv, fenv, _, prog) := t in
   let p := LambdaANF_to_Clight.compile
-             argsIdent allocIdent limitIdent gcIdent mainIdent bodyIdent threadInfIdent
+             argsIdent allocIdent limitIdent gcIdent mainIdent bodyIdent bodyName threadInfIdent
              tinfIdent heapInfIdent numArgsIdent isptrIdent caseIdent
              args p_env prog cenv nenv in
   match p with
@@ -52,19 +52,19 @@ Definition Clight_trans (prims : list (kername * string * bool * nat * positive)
 
 
 (* TODO unify with the one above, propagate errors *)
-Definition Clight_trans_fast (prims : list (kername * string * bool * nat * positive)) (args : nat) (t : toplevel.LambdaANF_FullTerm) : error Cprogram :=
+Definition Clight_trans_fast (bodyName : string) (prims : list (kername * string * bool * nat * positive)) (args : nat) (t : toplevel.LambdaANF_FullTerm) : error Cprogram :=
   let '(_, p_env, cenv, ctag, itag, nenv, fenv, _, prog) := t in
   let '(nenv, prog, head) := LambdaANF_to_Clight.compile_fast
-                               argsIdent allocIdent limitIdent gcIdent mainIdent bodyIdent threadInfIdent
+                               argsIdent allocIdent limitIdent gcIdent mainIdent bodyIdent bodyName threadInfIdent
                                tinfIdent heapInfIdent numArgsIdent isptrIdent caseIdent
                                args p_env prog cenv nenv in
   Ret (add_prim_names prims nenv, stripOption mainIdent prog, stripOption mainIdent head).
 
 
-Definition Clight_trans_ANF (prims : list (kername * string * bool * nat * positive)) (args : nat) (t : toplevel.LambdaANF_FullTerm) : error Cprogram * string :=
+Definition Clight_trans_ANF bodyName (prims : list (kername * string * bool * nat * positive)) (args : nat) (t : toplevel.LambdaANF_FullTerm) : error Cprogram * string :=
   let '(_, pr_env, cenv, ctag, itag, nenv, fenv, _, prog) := t in
   let '(p, str) := LambdaANF_to_Clight_stack.compile
-                     argsIdent allocIdent nallocIdent limitIdent gcIdent mainIdent bodyIdent threadInfIdent
+                     argsIdent allocIdent nallocIdent limitIdent gcIdent mainIdent bodyIdent bodyName threadInfIdent
                      tinfIdent heapInfIdent numArgsIdent isptrIdent caseIdent resultIdent
                      args
                      pr_env
@@ -85,6 +85,6 @@ Definition compile_Clight (prims : list (kername * string * bool * nat * positiv
     let args := c_args opts in
     let cps := negb (direct opts) in
     if cps then 
-      LiftErrorCertiCoqTrans "Codegen" (Clight_trans prims args) s
+      LiftErrorCertiCoqTrans "Codegen" (Clight_trans opts.(body_name) prims args) s
     else
-      LiftErrorLogCertiCoqTrans "Codegen" (Clight_trans_ANF prims args) s.
+      LiftErrorLogCertiCoqTrans "Codegen" (Clight_trans_ANF opts.(body_name) prims args) s.
